cp

Stlc/Nominal.v
@@ -1,37 +1,54 @@
-Require Import Metalib.Metatheory.
-Require Import Metalib.LibLNgen.
+(** A nominal representation of STLC terms.
 
-(* Some of our proofs are by induction on the *size* of
-   terms. We use the Omega tactic to easily dispatch reasoning
-   about natural numbers. *)
+    This version looks a lot like we expect a representation of
+    the lambda calculus to look like. Unlike the LN version,
+    the syntax does not distinguish between bound and free
+    variables and abstractions include the name of binding
+    variables.  *)
+
+(*************************************************************)
+(** * Imports                                                *)
+(*************************************************************)
+
+(** We will use the [atom] type from the metatheory library to
+    represent variable names. *)
+Require Export Metalib.Metatheory.
+
+(** Although we are not using LNgen, some of the tactics from
+    its library are useful for automating reasoning about
+    names.  *)
+Require Export Metalib.LibLNgen.
+
+(** Some of our proofs are by induction on the *size* of
+    terms. We'll use Coq's [omega] tactic to easily dispatch
+    reasoning about natural numbers. *)
 Require Export Omega.
 
-
 (*************************************************************)
-(*   A nominal representation of terms                       *)
+(** * A nominal representation of terms                      *)
 (*************************************************************)
-
-(* A named representation of STLC terms.
-
-   Binders include the names of free variables. *)
 
 Inductive n_exp : Set :=
- | n_var (x:var)
- | n_abs (x:var) (t:n_exp)
+ | n_var (x:atom)
+ | n_abs (x:atom) (t:n_exp)
  | n_app (t1:n_exp) (t2:n_exp).
 
-(* We can swap variables: this operation is
-   symmetric: x becomes y and y becomes x. *)
-Notation swap_var := (fun (x:var) (y:var) (z:var) =>
-  if (z == x) then y else if (z == y) then x else z).
+(** What makes this a *nominal* representation is that our
+    operations are based on the following swapping function for
+    names.  Note that this operation is symmetric: [x] becomes
+    [y] and [y] becomes [x]. *)
 
-(* The main insight of nominal representations:
+Definition swap_var (x:atom) (y:atom) (z:atom) :=
+  if (z == x) then y else if (z == y) then x else z.
 
-   We can rename variables, without capture, using a simple
-   structural induction. Note how the [n_abs} case
-   we swap all variables, both bound and free.
+Hint Unfold swap_var : nominal.
 
-   For example:
+(** The main insight of nominal representations is that we can
+    rename variables, without capture, using a simple
+    structural induction. Note how in the [n_abs] case we swap
+    all variables, both bound and free.
+
+    For example:
 
       (swap x y) (\z. (x y)) = \x. (y x))
 
@@ -40,15 +57,16 @@ Notation swap_var := (fun (x:var) (y:var) (z:var) =>
       (swap x y) (\y. x) = \x.y
 
 *)
-Fixpoint swap (x:var) (y:var) (t:n_exp) : n_exp :=
+Fixpoint swap (x:atom) (y:atom) (t:n_exp) : n_exp :=
   match t with
   | n_var z     => n_var (swap_var x y z)
   | n_abs z t1  => n_abs (swap_var x y z) (swap x y t1)
   | n_app t1 t2 => n_app (swap x y t1) (swap x y t2)
   end.
 
-(* The free variable function needs to remove the
-   bound variable in the [n_abs] case. *)
+
+(** The free variable function needs to remove the
+    bound variable in the [n_abs] case. *)
 Fixpoint fv_nom (n : n_exp) : atoms :=
   match n with
   | n_var x => {{x}}
@@ -56,16 +74,15 @@ Fixpoint fv_nom (n : n_exp) : atoms :=
   | n_app n1 n2 => fv_nom n1 `union` fv_nom n2
   end.
 
-(* We can also define the "alpha-equivalence" relation
-   that declares when two nominal terms are equivalent
-   (up to swapping).
+(** We can also define the "alpha-equivalence" relation that
+    declares when two nominal terms are equivalent (up to
+    renaming of bound variables).
 
-   Note the two different rules for [n_abs]: either the
-   binders are the same and we can directly compare the
-   bodies, or the binders differ, but we can swap one
-   side to make it look like the other.
+    Note the two different rules for [n_abs]: either the
+    binders are the same and we can directly compare the
+    bodies, or the binders differ, but we can swap one side to
+    make it look like the other.  *)
 
- *)
 Inductive aeq : n_exp -> n_exp -> Prop :=
  | aeq_var : forall x,
      aeq (n_var x) (n_var x)
@@ -82,105 +99,134 @@ Inductive aeq : n_exp -> n_exp -> Prop :=
 
 Hint Constructors aeq.
 
-(* -------------------------------------------------------- *)
+(*************************************************************)
+(** * Properties about swapping                              *)
+(*************************************************************)
 
-(* Properties about nominal terms. *)
 
-(* Some are straightforward to prove *)
+(** Because swapping is a simpl, structurally recursive
+    function, it is highly automatable using the [default_simp]
+    tactic from LNgen library.
+
+    This tactic "simplifies" goals using a combination of
+    common proof steps, including case analysis of all disjoint
+    sums in the goal. Because atom equality returns a sumbool,
+    this makes this tactic useful for reasoning by cases about
+    atoms.
+
+    For more information about the [default_simp] tactic, see
+    [metalib/LibDefaultSimp.v]. *)
 
 Lemma swap_id : forall n x,
     swap x x n = n.
 Proof.
-  induction n; default_simp.
+  induction n; simpl; unfold swap_var;  default_simp.
 Qed.
 
-Lemma swap_symmetric : forall n x y,
-    swap x y n = swap y x n.
-Proof.
-  induction n; default_simp.
-Qed.
-
-Lemma swap_involutive : forall n x y,
-    swap x y (swap x y n) = n.
-Proof.
-  induction n; default_simp.
-Qed.
-
-(* We will need these later! *)
+(** Demo: We will need the next two properties later in the tutorial,
+    so we show that even though there are many cases to consider,
+    [default_simp] can find these proofs. *)
 
 Lemma fv_nom_swap : forall z y n,
   z `notin` fv_nom n ->
   y `notin` fv_nom (swap y z n).
 Proof.
-  induction n; default_simp.
-Qed.
+  (* WORKINCLASS *)
+  induction n; intros; simpl; unfold swap_var; default_simp.
+Qed. (* /WORKINCLASS *)
 
 Lemma shuffle_swap : forall w y n z,
     w <> z -> y <> z ->
     (swap w y (swap y z n)) = (swap w z (swap w y n)).
 Proof.
-  induction n; default_simp.
-Qed.
+  (* WORKINCLASS *)
+  induction n; intros; simpl; unfold swap_var; default_simp.
+Qed. (* /WORKINCLASS *)
 
-(* Other proofs about nominal terms involve swapping to make sure that
-   variable names are "fresh enough". In this case, we need to strengthen our
-   induction hypothesis.
- *)
+(*************************************************************)
+(** * Exercises                                              *)
+(*************************************************************)
 
-Fixpoint size (n : n_exp) : nat :=
-  match n with
-  | n_var x => 1
-  | n_abs x e => 1 + size e
-  | n_app e1 e2 => 1 + size e1 + size e2
-  end.
 
-Lemma swap_size_constant : forall x y n,
-    size (swap x y n) = size n.
+(** Exercise: swap properties
+
+    Prove the following properties about swapping, either
+    explicitly (by destructing [x == y]) or automatically
+    (using [default_simp]).  *)
+
+Lemma swap_symmetric : forall n x y,
+    swap x y n = swap y x n.
 Proof.
-  induction n; simpl; auto.
-Qed.
+  (* ADMITTED *)
+  induction n;  simpl; unfold swap_var; default_simp.
+Qed.   (* /ADMITTED *)
 
-Hint Rewrite swap_size_constant.
-
-
-Local Ltac gather_atoms ::=
-  let A := gather_atoms_with (fun x : atoms => x) in
-  let B := gather_atoms_with (fun x : atom => singleton x) in
-  let D := gather_atoms_with (fun x : n_exp => fv_nom x) in
-  constr:(A `union` B `union` D).
-
-Lemma nominal_induction_size L :
-     forall n, forall t, size t <= n ->
-     forall P : n_exp -> Prop,
-    (forall x, P (n_var x)) ->
-    (forall x t, (forall y, y `notin` L -> P (swap x y t)) -> P (n_abs x t)) ->
-    (forall t1 t2, P t1 -> P t2 -> P (n_app t1 t2)) ->
-    P t.
+Lemma swap_involutive : forall n x y,
+    swap x y (swap x y n) = n.
 Proof.
-  induction n.
-  intros t SZ; destruct t; simpl in *; inversion SZ.
-  intros t SZ P VAR ABS APP; destruct t; simpl in *.
-  - auto.
-  - apply ABS.
-    intros y Fr.
-    apply IHn; eauto; rewrite swap_size_constant; try omega.
-  - apply APP.
-    apply IHn; eauto; omega.
-    apply IHn; eauto; omega.
-Qed.
+  (* ADMITTED *)
+  induction n;  simpl; unfold swap_var; default_simp.
+Qed.   (* /ADMITTED *)
 
-Definition nominal_induction
-  : forall (L : atoms) (P : n_exp -> Prop),
-    (forall x : atom, P (n_var x)) ->
-    (forall (x : atom) (t : n_exp),
-        (forall y : atom, y `notin` L -> P (swap x y t)) -> P (n_abs x t)) ->
-    (forall t1 t2 : n_exp, P t1 -> P t2 -> P (n_app t1 t2)) ->
-    forall t : n_exp, P t :=
-  fun L P VAR APP ABS t =>
-  nominal_induction_size L (size t) t ltac:(auto) P VAR APP ABS.
+(** Challenge exercises: equivariance
 
-(* -------------------------------------------------------- *)
-(* An abstract machine for cbn evaluation of named terms    *)
+    Equivariance is the property that all functions and relations
+    are preserved under swapping.
+
+*)
+Lemma swap_var_equivariance : forall n x y z w,
+    swap_var x y (swap_var z w n) =
+    swap_var (swap_var x y z) (swap_var x y w) (swap_var x y n).
+Proof.
+  (* ADMITTED *)
+  unfold swap_var; default_simp.
+Qed.   (* /ADMITTED *)
+
+Lemma swap_equivariance : forall n x y z w,
+    swap x y (swap z w n) = swap (swap_var x y z) (swap_var x y w) (swap x y n).
+Proof.
+  (* ADMITTED *)
+  induction n; intros; simpl.
+  - rewrite swap_var_equivariance. auto.
+  - rewrite swap_var_equivariance. rewrite IHn. auto.
+  - rewrite IHn1. rewrite IHn2. auto.
+Qed. (* /ADMITTED *)
+
+Lemma fv_nom_equivariance : forall x0 x y n,
+  x0 `notin` fv_nom n ->
+  swap_var x y x0  `notin` fv_nom (swap x y n).
+Proof.
+  (* ADMITTED *)
+  induction n; intros; simpl in *.
+  - unfold swap_var; default_simp.
+  - unfold swap_var in *. default_simp.
+  - destruct_notin.
+    eapply IHn1 in H.
+    eapply IHn2 in NotInTac.
+    fsetdec.
+Qed. (* /ADMITTED *)
+
+Lemma aeq_equivariance : forall x y n1 n2,
+    aeq n1 n2 ->
+    aeq (swap x y n1) (swap x y n2).
+Proof.
+  (* ADMITTED *)
+  induction 1; intros; simpl in *; auto.
+  destruct (swap_var x y x0 == swap_var x y y0).
+  - rewrite e. eapply aeq_abs_same.
+    rewrite swap_equivariance in IHaeq.
+    rewrite e in IHaeq.
+    rewrite swap_id in IHaeq.
+    auto.
+  - rewrite swap_equivariance in IHaeq.
+    eapply aeq_abs_diff; auto.
+    eapply fv_nom_equivariance; auto.
+Qed. (* /ADMITTED *)
+
+(*************************************************************)
+(** * An abstract machine for cbn evaluation                 *)
+(*************************************************************)
+
 
 Fixpoint get {A :Type} (x:atom) (l : list (atom * A)) : option A :=
   match l with
@@ -189,14 +235,30 @@ Fixpoint get {A :Type} (x:atom) (l : list (atom * A)) : option A :=
   end.
 
 
-(* The advantage of named terms is an efficient operational semantics! We
-   don't need to recurse terms, opening and closing each binder. Instead, as
-   long as the binder is "sufficiently fresh" we can use the name as is, and
-   only rename (via swapping) when absolutely necessary. *)
+(** The advantage of named terms is an efficient operational
+    semantics! Compared to LN or debruijn representation, we
+    don't need to modify terms (such as via open or shifting)
+    as we traverse binders. Instead, as long as the binder is
+    "sufficiently fresh" we can use the name as is, and only
+    rename (via swapping) when absolutely necessary. *)
 
-(* We also don't even need to use substitution for our semantics.  Our
-   abstract maching will work with configurations (see below) which consist of
-   a head (i.e. delayed substitution) a term, and a stack. *)
+(** Below, we define an operational semantics based on an
+    abstract machine.
+
+    Our abstract machine configurations have three components:
+
+    - the current expression being evaluated
+    - the heap (aka environment):
+        a mapping between variables and expressions
+    - the stack:
+        the evaluation context of the current expression
+
+    Because we have a heap, we don't need to use substitution
+    to define our semantics! To implement [e/x] we place e on
+    the heap and then look it up when we get to x during
+    evaluation.
+*)
+
 
 Definition heap := list (atom * n_exp).
 
@@ -205,13 +267,12 @@ Notation  stack := (list frame).
 
 Definition conf := (heap * n_exp * stack)%type.
 
+(** The (small-step) semantics is a function from configurations to
+    configurations, until completion or error. *)
 
-(* The (small-step) semantics is a function from configurations to
-   configurations, until completion or error. *)
-
-Inductive Step a := Error   : Step a
-                 | Done     : Step a
-                 | TakeStep : a -> Step a.
+Inductive Step a := Error    : Step a
+                  | Done     : Step a
+                  | TakeStep : a -> Step a.
 
 Definition isVal (e : n_exp) :=
   match e with
@@ -250,24 +311,249 @@ Definition machine_step (avoid : atoms) (c : conf) : Step conf :=
 Definition initconf (e : n_exp) : conf := (nil,e,nil).
 
 
-(*
+(** Example: evaluation of  "(\y. (\x. x) y) X"
 
-Example: evaluation of  "(\y. (\x. x) y) 0"
-
+<<
      machine                                       corresponding term
 
-      {}, (\y. (\x. x) y) 0 , nil                  (\y. (\x. x) y) 0
-  ==> {}, (\y. (\x. x) y), n_app2 0 :: nil         (\y. (\x. x) y) 0
-  ==> {y -> 0}, (\x.x) y, nil                      (\x. x) 0
-  ==> {y -> 0}, (\x.x), n_app2 y :: nil            (\x. x) 0
-  ==> {y -> 0}, y , nil                            0
-  ==> {y -> 0}, 0 , nil                            0
+      {}, (\y. (\x. x) y) X , nil                  (\y. (\x. x) y) X
+  ==> {}, (\y. (\x. x) y), n_app2 X :: nil         (\y. (\x. x) y) X
+  ==> {y -> X}, (\x.x) y, nil                      (\x. x) X
+  ==> {y -> X}, (\x.x), n_app2 y :: nil            (\x. x) X
+  ==> {y -> X}, y , nil                            X
+  ==> {y -> X}, X , nil                            X
   ==> Done
+>>
 
 (Note that the machine takes extra steps compared to the
 substitution semantics.)
 
 *)
+
+
+(*************************************************************)
+(** * Size, Nominal induction and recursion                  *)
+(*************************************************************)
+
+
+(** Some properties about nominal terms require calling the
+    induction hypothesis not on a direct subterm, but on one
+    that has first had a swapping applied to it.
+
+    However, swapping names does not change the size of terms,
+    so that means we can prove such properties by induction on
+    that size.  *)
+
+Fixpoint size (n : n_exp) : nat :=
+  match n with
+  | n_var x => 1
+  | n_abs x e => 1 + size e
+  | n_app e1 e2 => 1 + size e1 + size e2
+  end.
+
+Lemma swap_size_eq : forall x y n,
+    size (swap x y n) = size n.
+Proof.
+  induction n; simpl; auto.
+Qed.
+
+Hint Rewrite swap_size_eq.
+
+
+Lemma nominal_induction_size L :
+     forall n, forall t, size t <= n ->
+     forall P : n_exp -> Type,
+    (forall x, P (n_var x)) ->
+    (forall x t, (forall y, y `notin` L -> P (swap x y t)) -> P (n_abs x t)) ->
+    (forall t1 t2, P t1 -> P t2 -> P (n_app t1 t2)) ->
+    P t.
+Proof.
+  induction n.
+  intros t SZ; destruct t; intros; simpl in SZ; omega.
+  intros t SZ P VAR ABS APP; destruct t; simpl in *.
+  - auto.
+  - apply ABS.
+    intros y Fr.
+    apply IHn; eauto; rewrite swap_size_eq; try omega.
+  - apply APP.
+    apply IHn; eauto; omega.
+    apply IHn; eauto; omega.
+Defined.
+
+Definition nominal_induction
+  : forall (L : atoms) (P : n_exp -> Type),
+    (forall x : atom, P (n_var x)) ->
+    (forall (x : atom) (t : n_exp),
+        (forall y : atom, y `notin` L -> P (swap x y t)) -> P (n_abs x t)) ->
+    (forall t1 t2 : n_exp, P t1 -> P t2 -> P (n_app t1 t2)) ->
+    forall t : n_exp, P t :=
+  fun L P VAR APP ABS t =>
+  nominal_induction_size L (size t) t ltac:(auto) P VAR APP ABS.
+
+(* LATER *)
+
+Definition extract {L} (m : {x : atom | x `notin` L}) : atom :=
+  match m with
+  | exist _ x _ => x
+  end.
+
+Inductive subst_rel (u : n_exp) (x: atom) : n_exp -> n_exp -> Prop :=
+ | subst_var_same : subst_rel u x (n_var x) u
+ | subst_var_diff : forall y, x <> y -> subst_rel u x (n_var y) (n_var y)
+ | subst_abs      : forall y z t0 t0',
+     z = extract (atom_fresh (fv_nom u \u fv_nom (n_abs y t0))) ->
+     subst_rel u x (swap y z t0) t0' ->
+     subst_rel u x (n_abs y t0) (n_abs z t0')
+ | subst_app      : forall t0 t0' t1 t1',
+     subst_rel u x t0 t0' ->
+     subst_rel u x t1 t1' ->
+     subst_rel u x (n_app t0 t1) (n_app t0' t1').
+Hint Constructors subst_rel.
+
+
+Lemma subst_rel_exists : forall u x t, sig (subst_rel u x t).
+Proof.
+  intros u x t.
+  apply nominal_induction with (t := t)(L := fv_nom u).
+  - intros y. destruct (x == y); subst. exists u. eauto.
+    exists (n_var y). auto.
+  - intros y t0 IH.
+    remember (atom_fresh (fv_nom u \u fv_nom (n_abs y t0))) as sg.
+    destruct (IH (extract sg)) as [t0' K]. subst. simpl.
+    unfold extract. destruct atom_fresh.
+    fsetdec.
+    exists (n_abs (extract sg) t0'). subst; eauto.
+  - intros t1 t2 [t1' IH1] [t2' IH2].
+    exists (n_app t1' t2'). eauto.
+Defined.
+
+Definition subst (u : n_exp) (x:atom) (t:n_exp) : n_exp :=
+  match (subst_rel_exists u x t) with
+  | exist _ t' _ => t'
+  end.
+
+Lemma simpl_subst_app : forall u x t1 t2,
+    subst u x (n_app t1 t2) = n_app (subst u x t1) (subst u x t2).
+Proof.
+  intros.
+  unfold subst in *.
+  destruct subst_rel_exists.
+  inversion s.
+Admitted.
+
+
+Program Fixpoint subst_rec (n:nat) (t:n_exp) (pf : size t <= n)
+        (u :n_exp) (x:atom)  : n_exp :=
+  match n with
+  | 0 => _
+  | S m => match t with
+          | n_var y => if (x == y) then u else t
+          | n_abs y t1 => if (x == y) then t
+                        else let (z,_) := atom_fresh (fv_nom u \u fv_nom t) in
+                             n_abs z (subst_rec m (swap y z t1) _ u x)
+          | n_app t1 t2 => n_app (subst_rec m t1 _ u x) (subst_rec m t2 _ u x)
+          end
+  end.
+Next Obligation.
+rewrite swap_size_eq. simpl in *. omega.
+Defined.
+Next Obligation.
+simpl in *. omega.
+Defined.
+Next Obligation.
+simpl in *. omega.
+Defined.
+
+Lemma subst_rec_proof_irrel :
+  forall n t p1 p2 u x, subst_rec n t p1 u x = subst_rec n t p2 u x.
+Proof.
+  induction n.
+  simpl. auto.
+  simpl. destruct t; auto.
+  - intros; destruct (x0 == x); auto.
+    destruct atom_fresh; auto.
+    erewrite IHn. eauto.
+  - intros.
+    erewrite IHn with (t := t1).
+    erewrite IHn with (t := t2).
+    eauto.
+Qed.
+
+(* /LATER *)
+
+(*
+Lemma subst_rec_size_weaken :
+  forall n1 t u x (p1 : size t <= n1) (p2: size t <= size t),
+    subst_rec n1 t p1 u x = subst_rec (size t) t p2 u x.
+Proof.
+  induction n1.
+  intros. destruct t; simpl in p1; omega.
+  intros. destruct t.
+  - simpl in *. auto.
+  - simpl in *.
+    destruct (x == x0); subst; auto.
+    destruct atom_fresh; auto.
+    replace (size t) with (size (swap x0 x1 t)).
+    erewrite IHn1.
+
+
+  -
+
+
+Definition subst (u : n_exp) (x:atom) (t:n_exp) :=
+  subst_rec (size t) t ltac:(auto) u x.
+
+Lemma subst_var_eq : forall u x,
+    subst u x (n_var x) = u.
+Proof.
+  intros. unfold subst. default_simp.
+Qed.
+Lemma subst_var_neq : forall u x y,
+    x <> y ->
+    subst u x (n_var y) = n_var y.
+Proof.
+  intros. unfold subst. default_simp.
+Qed.
+Lemma subst_app : forall u x t1 t2,
+    subst u x (n_app t1 t2) = n_app (subst u x t1) (subst u x t2).
+Proof.
+  intros. unfold subst.
+  erewrite subst_rec_proof_irrel with (t := t1).
+  erewrite subst_rec_proof_irrel with (t := t2).
+  simpl; eauto.
+  remember (le_n (size (n_app t1 t2))) as Pf1.
+  remember (le_n (size t1)) as Pf2.
+  remember (le_n (size t2)) as Pf3.
+  simpl.
+
+  repeat f_equal. f_equal.
+
+Definition impossible {A:Type} (t:n_exp)(pf: size t <= 0) : A.
+destruct t; simpl in pf; omega.
+Defined.
+
+Fixpoint nominal_recursion_size {A : Type} L
+  (n : nat) (t : n_exp) (pf : size t <= n)
+          (VAR : atom -> A)
+          (ABS : forall x, x `notin` L -> A -> A)
+          (APP : A -> A -> A)
+           : A :=
+  match n with
+  | 0 => impossible t _
+  | S m => match t with
+          | n_var x => VAR x
+          | n_abs y t0 =>
+            let (z,Pf) := atom_fresh L in
+            let ABS'   := fun x Fr => ABS x _ in
+            ABS z Pf (nominal_recursion_size
+                        (add z L) m (swap z y t0) _ VAR ABS' APP)
+          | n_app t0 t1 =>
+            APP (nominal_recursion_size L m t0 _ VAR ABS APP)
+                (nominal_recursion_size L m t1 _ VAR ABS APP)
+          end
+  end.
+*)
+
 
 (*
 Inductive typ := typ_base | typ_arrow : typ -> typ -> typ.
@@ -331,3 +617,42 @@ Proof.
       instantiate (1 :=  [(x0,T3)] ++ G).
       eapply typing_heap_cons; eauto.
 *)
+
+Lemma aeq_fv_nom : forall n1 n2,
+    aeq n1 n2 ->
+    fv_nom n1 [=] fv_nom n2.
+Proof.
+  induction 1; simpl in *; try fsetdec.
+  rewrite IHaeq.
+  apply fv_nom_equivariance with (x:=x)(y:=y) in H0.
+  unfold swap_var in H0. default_simp.
+Admitted.
+
+Lemma aeq_refl : forall n, aeq n n.
+Proof.
+  induction n; auto.
+Qed.
+
+Lemma aeq_sym : forall n1 n2,
+    aeq n1 n2 -> aeq n2 n1.
+Proof.
+  induction 1; auto.
+  - eapply aeq_abs_diff; auto.
+    admit.
+    eapply aeq_equivariance in IHaeq.
+    rewrite swap_involutive in IHaeq.
+    rewrite swap_symmetric.
+    auto.
+Admitted.
+
+Lemma aeq_trans : forall n2 n1 n3, aeq n1 n2 -> aeq n2 n3 -> aeq n1 n3.
+Proof.
+  induction n2; intros; simpl in *.
+  - inversion H; inversion H0. subst. auto.
+  - inversion H; inversion H0; subst; auto.
+    eapply aeq_abs_diff; eauto.
+    rewrite <- aeq_fv_nom; eauto.
+    assert (aeq (swap x x0 n2) (swap x x0 n6)).
+    eapply aeq_equivariance; auto.
+    admit. (* sized based ih *)
+Admitted.
